<section xml:id="section-parts">
  <title>Integration by Parts</title>
  <subsection xml:id="subsection-parts-definition">
    <title>Definition</title>
    <p>
      In this section, I am going to try to invert the product rule
      for derivatives to build a new rule for integration. First,
      recall the product rule, for <m>f(x)</m> and <m>g(x)</m>
      differentiable functions. 
    </p>
    <me>
      \frac{d}{dx} f(x) g(x) = \frac{df}{dx} g(x) + f(x)
      \frac{dg}{dx}
    </me>
    <p>
      I'm simply going to integrate both sides of this equation. On
      the left, the integral of a derivative returns the  original
      function. (I'll simplify the notation from <m>f(x)</m> to
      just <m>f</m>; this is a very common notation shift that makes
      some of these more compicated integration rules a bit more
      succinct. It's just up to you to remember that <m>f</m> and
      <m>g</m> are functions.) 
    </p>
    <md>
      <mrow>
        \int \frac{d}{dx} fg dx \amp = \int \frac{df}{dx} g dx
        + \int f \frac{dg}{dx} dx
      </mrow>
      <mrow>
        fg \amp = \int \frac{df}{dx} g dx + \int f
        \frac{dg}{dx} dx
      </mrow>
    </md>
    <p>
      This is a rule about integrals, but it's not clear how to use
      it. I'm going to isolate one of the two integral pieces. 
    </p>
    <me>
      \int \frac{df}{dx} g dx = fg - \int f \frac{dg}{dx} dx
    </me>
    <p>
      This might be more useful, since it tells me how to transform
      certain integral. This is useful enough that there is a name for
      it. 
    </p>
    <definition>
      <statement>
        <p>
          Let <m>f</m> and <m>g</m> be functions, with <m>f</m>
          integrable and <m>g</m> differentiable. The following
          equation for the integral of <m>\frac{df}{dx} g</m> is
          called <term>integration by parts</term>.
        </p>
        <me>
          \int \frac{df}{dx} g dx = fg - \int f \frac{dg}{dx} dx
        </me>
      </statement>
    </definition>
    <p>
      So how do I actually use this? The left side of integration by
      parts is a product: <m>\frac{df}{dx} g</m>. Integration by parts
      applies to integals of product. However, I have to identify one
      part of the product as <m>g</m> and another part as
      <m>\frac{df}{dx}</m>. Then, I need to calculate
      <m>\frac{dg}{dx}</m>, a derivative, and <m>f</m>, an
      antiderivative. If I can do these two things for the choice I
      made, then I can transfer to the right side of integration by
      parts. The first part, <m>fg</m> is just a function, but the
      second part is a new integral, with integrand <m>f
      \frac{dg}{dx}</m>. Maybe this is an easier integral. Like the
      substitution rule, integration by parts doesn't solve the
      integral by itself; instead, it changes the form of the integral
      into something which is (hopefully) more approachable.
    </p>
    <p>
      In applying the substitution rule, I encouraged careful
      labelling. The same is true here: I recommend labelling the
      terms and being particularly careful with <m>\pm</m> signs. In
      other literature, there are some concise version of integration
      by parts with slightly different notations (using <m>df</m> and
      <m>dg</m> for the integrals). I'm not going to use that notation,
      but for reference, here is what the rule looks like. 
    </p>
    <me>
      \int g df = fg - \int f dg
    </me>
    <p>
      If I have a definite integral, I can still use integration by
      parts. On the middle term (the term which is not an integral), I
      have to evalute on the bounds. 
    </p>
    <me>
      \int_a^b \frac{df}{dx} g(x) dx = f(x)g(x) \Bigg|_a^b  - \int_a^b
      f(x) \frac{dg}{dx} dx 
    </me>
  </subsection>
  <subsection xml:id="parts-examples">
    <title>Examples</title>
    <example>
      <statement>
        <p>
          The first step in any integration by parts is chooing which
          piece is <m>f</m> and which is <m>g</m>.
          In this integral, one choice makes the following integral
          easier and one makes it more difficult. The first choice I
          might make is <m>\frac{df}{dx} = x</m> and <m>g = e^x</m>.
          <md>
            <mrow>
              \int x e^x dx \amp
            </mrow>
            <mrow>
              \frac{df}{dx} \amp = x \implies f = \frac{x^2}{2}
            </mrow>
            <mrow>
              g \amp = e^x \implies \frac{dg}{dx} = e^x
            </mrow>
            <mrow>
              \int x e^x dx \amp = \frac{x^2}{2} e^x - \int
              \frac{x^2}{2} e^x dx
            </mrow>
          </md>
        </p>
        <p>
          This gives a new integral which isn't any easier than the
          previous. This use of integration by parts hasn't helped.
          Instead, I'll try <m>\frac{df}{dx} = e^x</m> and <m>g = x</m>.
          <md>
            <mrow>
              \int x e^x dx \amp
            </mrow>
            <mrow>
              \frac{df}{dx} \amp = e^x \implies f = e^x
            </mrow>
            <mrow>
              g \amp = x \implies \frac{dg}{dx} = 1
            </mrow>
            <mrow>
              \int x e^x dx \amp = xe^x - \int e^x dx = xe^x - e^x + c
              = (x-1)e^x + c
            </mrow>
          </md>
        </p>
        <p>
          This choice worked, and I was able to continue on to the
          complete solution. As with all integration problems, I can
          check my answer by differentiation.
          <me>
            \frac{d}{dx} (x-1)e^x + c = e^x \frac{d}{dx} (x-1) + (x-1)
            \frac{d}{dx} e^x = e^x + xe^x - e^x = xe^x
          </me>
        </p>
      </statement>
    </example>
    <example>
      <statement>
        <p>
          For integration by parts, I choose <m>g = x</m> and
          <m>\frac{df}{dx} = \cos x</m>, since finding the
          antiderivative of the cosine is easy and the derivate of
          <m>x</m> is just a constant.  This choice should simplify
          the integral.
        </p>
        <md>
          <mrow>
            \int x \cos x dx \amp
          </mrow>
          <mrow>
            \frac{df}{dx} \amp = \cos x \implies f = \sin x
          </mrow>
          <mrow>
            g \amp = x \implies \frac{dg}{dx} = 1
          </mrow>
          <mrow>
            \int x \cos x dx \amp = x \sin x - \int \sin x dx = (x \sin x +
          \cos x) + c
        </mrow>
        </md>
        <p>
          The choice did indeed simplify the integral, leaving only
          <m>\sin x</m> in the integral. 
        </p>
      </statement>
    </example>
    <example>
      <statement>
        <p>
          This example uses integration by parts twice. Pay attention
          to the <m>\pm</m> signs. In the first step, I choose <m>g
          = x^2</m> and <m>\frac{df}{dx} = e^x</m>. 
        </p>
        <md>
          <mrow>
            \int x^2 e^x dx \amp 
          </mrow>
          <mrow>
            \frac{df}{dx} \amp = e^x \implies f = e^x
          </mrow>
          <mrow>
            g \amp = x^2 \implies \frac{dg}{dx} = 2x 
          </mrow>
          <mrow>
            \int x^2 e^x dx \amp = x^2 e^x - \int 2x e^x dx
          </mrow>
        </md>
        <p>
          Now I do integration by parts again on the remaining
          integral. I choose <m>g = 2x</m> and <m>\frac{df}{dx} =
          e^x</m>, so that <m>\frac{dg}{dx} = 2</m> and <m>f =
          e^x</m>.
        </p>
        <md>
          <mrow>
            x^2 e^x - \int 2x e^x \amp = x^2 e^x - \left( 2xe^x - \int 2e^x
            dx \right)
          </mrow>
          <mrow>
            \amp = x^2 e^x - 2xe^x + 2e^x + c
          </mrow>
        </md>
      </statement>
    </example>
    <example>
      <statement>
        <p>
          In this example, I choose <m>g = x</m> and
          <m>\frac{df}{dx} = e^x</m>, which leads to <m>\frac{dg}{dx}
          = 1</m> and <m>f = e^x</m>. Since this is a definite
          integral, I need to evalute the bounds on the resulting
          middle term. After integration by parts, the remaining
          integral is a simple antiderivative.
        </p>
        <me>
          \int_1^2 x e^x dx = xe^x \Bigg|_1^2 - \int_1^2 e^x dx = 2e^2
          - e - e^x \Bigg|_1^2 = 2e^2 - e - e^2 + e = e^2
        </me>
      </statement>
    </example>
    <example>
      <statement>
        <p>
          In this example, I choose <m>\frac{df}{dx} = x^2</m> and
          <m>g = \ln x</m>. Since this is a definite integral, I
          evaluate the middle term on the bounds of the integral. 
          <md>
            <mrow>
              \int_1^{e^2} x^2 \ln x dx \amp = \frac{x^3}{3}
              \ln x \Bigg|_1^{e^2} - \int_1^{e^2} \frac{x^3}{3}
              \frac{1}{x} dx
            </mrow>
            <mrow>
              \amp = \frac{e^6}{3} 2 - \frac{1}{3} 0 - \frac{1}{3}
              \int_1^{e^2} x^2 dx = \frac{2e^6}{3} - \frac{x^3}{9}
              \Bigg|_1^{e^2}
            </mrow>
            <mrow>
              \amp = \frac{2e^6}{3} - \frac{e^6}{9} + \frac{1}{9} =
              \frac{5e^6 + 1}{9}
            </mrow>
          </md>
        </p>
      </statement>
    </example>
    <example>
      <statement>
        <p>
          The next integrand doesn't look anything like a product, but
          I can still use integration by parts by making a very clever
          choice of the functions. I choose <m>g = \ln x</m> and
          <m>\frac{df}{dx}= 1</m> which leads to <m>f = x</m> and
          <m>\frac{dg}{dx} = \frac{1}{x}</m>.
        </p>
        <me>
          \int \ln x dx = x \ln x - \int \frac{x}{x} dx = x \ln x -
          \int 1 dx = x \ln x - x + c
        </me>
      </statement>
    </example>
    <example>
      <statement>
        <p>
          This example is a clever and tricky use of integration by
          parts to deal with an important but difficult types of
          integral. Let <m>a,b \in \RR</m> with <m>a,b \neq 0</m>. In
          the following integral, I am going to use integration by
          parts twice in a row.
        </p>
        <md>
          <mrow>
            \int e^{ax} \sin bx dx \amp
          </mrow>
          <mrow>
            \frac{df}{dx} \amp = e^{ax} \implies f = \frac{e^{ax}}{a}
          </mrow>
          <mrow>
            g \amp = \sin bx \implies \frac{dg}{dx} = b \cos bx
          </mrow>
          <mrow>
            \int e^{ax} \sin bx dx \amp = \frac{e^{ax} \sin bx}{a}
            - \int \frac{b}{a} e^{ax} \cos bx dx
          </mrow>
          <mrow>
            \frac{df}{dx} \amp = e^{ax} \implies f = \frac{e^{ax}}{a}
          </mrow>
          <mrow>
            g \amp = \cos bx \implies \frac{dg}{dx} = -b \sin bx
          </mrow>
          <mrow>
            \amp = \frac{e^{ax}\sin bx}{a} - \frac{b}{a} \left(
            \frac{e^{ax} \cos bx}{a} - \int \frac{b}{a} e^{ax}
            (-\sin bx) dx \right)
          </mrow>
          <mrow>
            \int e^{ax} \sin bx dx \amp
            = \frac{e^{ax}\sin bx}{a} - \frac{be^{ax} \cos
            bx}{a^2} - \frac{b^2}{a^2} \int e^{ax} \sin bx dx
          </mrow>
        </md>
        <p>
          What have I accomplished? I've done integration by parts
          twice, but all I've done is returned back to the original
          integral. This seems like a dead end, but I can actually
          solve the integral from this equation. I'll add
          whole last term on the right from both sides of the
          equation, to cancel it from the right and add it to the
          left.
        </p>
        <me>
          \int e^{ax} \sin bx dx - \frac{b^2}{a^2} \int e^{ax} \sin
          bx dx = \frac{e^{ax}\sin bx}{a} - \frac{be^{ax} \cos
          bx}{a^2} 
        </me>
        <p>
          Now I'll rewrite the left side, factoring out the common
          integral term from both pieces. After doing that, I can
          divide by the resulting non-integral term. 
        </p>
        <md>
          <mrow>
            \left( 1 + \frac{b^2}{a^2} \right) \int e^{ax} \sin bx
            dx \amp = \frac{ae^{ax} \sin b x - b e^{ax} \cos
            bx}{a^2}
          </mrow>
          <mrow>
            \int e^{ax} \sin bx dx \amp = \frac{\frac{ae^{ax} \sin
            b x - b e^{ax} \cos bx}{a^2}}{\frac{a^2+b^2}{a^2}}
          </mrow>
          <mrow>
            \int e^{ax} \sin bx dx \amp = \frac{ae^{ax} \sin b x -
            b e^{ax} \cos bx}{a^2+b^2}
          </mrow>
        </md>
        <p>
          The result is an expression for the antiderivative of this
          difficult function. 
        </p>
      </statement>
    </example>
    <example>
      <statement>
        <p>
          Some integrals need a combination of techniques and rules.
          Here, I'm first going to do a substitution, using <m> u =
          \sqrt{x}</m> with <m>du = \frac{1}{2\sqrt{x}} dx</m>. By
          changing <m>\sqrt{x}</m> yto <m>u</m>, I can write this as
          <m>2udu = dx</m>, allowing me to directly replace the
          <m>dx</m>. The bounds will change as well, with <m>x = 0</m>
          becoming <m>u = \sqrt{0} = 0</m> and <m>x =
          \frac{\pi^2}{4}</m> bcoming <m>u = \sqrt{\frac{\pi^2}{4}} =
          \frac{\pi}{2}</m>.
        </p>
        <me>
          \int_0^{\frac{\pi^2}{4}} \sin \sqrt{x} dx =
          \int_0^{\frac{\pi}{2}} 2u \sin u du 
        </me>
        <p>
          then I'm going to use integration by parts to solve the
          integral that results from the substitution. I will choose
          <m>\frac{df}{du} = \sin u</m> and <m>g = 2u </m>, which
          leads to <m>f = -\cos u</m> and <m>\frac{dg}{du} = 2</m>.
          Since this is a definite integral, I'll evaluate the middle
          non-integral term on the bounds. 
        </p>
        <md>
          <mrow>
            \int_0^{\frac{\pi}{2}} 2u \sin u du \amp = 2u (-\cos u)
            \Bigg|_0^{\frac{\pi}{2}} - \int_0^{\frac{\pi}{2}} 2 (-\cos
            u) du
          </mrow>
          <mrow>
            \amp = 2 \frac{\pi}{2} \left( -\cos \frac{\pi}{2}
            \right) + 2 \int_0^{\frac{\pi}{2}} \cos u du = 2 \sin u
            \Bigg|_0^{\frac{\pi}{2}} = 2
          </mrow>
        </md>
      </statement>
    </example>
  </subsection>
</section>
