<section xml:id="quadratic-types">
  <title>Quadratic Types in Partial Fractions</title>
  <subsection xml:id="irreducible-factors">
    <title>Irreducible Factors</title>
    <example>
      <statement>
        <p>
          Here is an example with an irreducible factor.
          <me>
            \int \frac{x^2-x-1}{x^3-3x^2+5x-3} dx
          </me>
        </p>
        <p>
          The denominator has <m>x=1</m> as a root and it factors as <m>(x-1)(x^2-2x+3)</m>.
          The discriminant of the quadratic is <m>-8</m>,
          so it is irreducible and cannot be factored any further.
          Therefore, we are looking for a partial fraction decomposition of the following form.
          <me>
            \frac{x^2- x - 1}{x^3-3x^2+5x+3} = \frac{a}{x-1} + \frac{bx+c}{x^2-2x+3}
          </me>
        </p>
        <p>
          We take the right side to common denominator.
          <md>
            <mrow>\frac{x^2- x - 1}{x^3-3x^2+5x+3} \amp  = \frac{a}{x-1} + \frac{bx+c}{x^2-2x+3}</mrow>
            <mrow>\amp  = \frac{a(x^2 - 2x + 3) + (bx+c)(x-1)}{x^3-3x^2+5x-3}</mrow>
            <mrow>\amp  = \frac{ax^2 - 2ax + 3a + bx^2 - bx + cx -c}{x^3-3x^2+5x-3}</mrow>
            <mrow>\amp  = \frac{(a+b)x^2 + (-2a-b+c)x + (3a-c)}{x^3-3x^2+5x-3}</mrow>
          </md>
        </p>
        <p>
          That gives a system with <m>a+b=1</m>,
          <m>-2-b+c=-1</m> and <m>3a-c=-1</m>.
          We can use the first and third equations to write everything in terms of <m>a</m>.
          That gives <m>b = 1-a</m> and <m>c = 3a+1</m>.
          We replace both in the second equation.
          <md>
            <mrow>-2a + (1-a) + (3a + 1) \amp  = -1</mrow>
            <mrow>-2a -1 + a + 3a + 1 \amp  = -1</mrow>
            <mrow>2a \amp  = -1 \implies a = \frac{-1}{2}</mrow>
            <mrow>b \amp  = 1 - \frac{-1}{2} = \frac{3}{2}</mrow>
            <mrow>c \amp  = 3 \frac{-1}{2} + 1 = \frac{-1}{2}</mrow>
          </md>
        </p>
        <p>
          This finishes the partial fraction decomposition.
          <me>
            \frac{x^2-x-1}{x^3-3x^2+5x-3} = \frac{\frac{-1}{2}}{x-1} + \frac{\frac{3}{2} x - \frac{-1}{2}}{x^2 - 2x +3}
          </me>
        </p>
        <p>
          Then we can integrate.
          <me>
            \int \frac{x^2-x-1}{x^3-3x^2+5x-3} dx = \frac{-1}{2} \int \frac{1}{x-1} dx + \int \frac{\frac{3}{2} x - \frac{-1}{2}}{x^2 - 2x +3} dx
          </me>
        </p>
        <p>
          The first term is easy, but now we have a quadratic term.
          We solve the quadratic by isolating a piece of it which allows for a substitution,
          and completing the square on the remaining pieces and using an arctan integral.
          <md>
            <mrow>\amp  \int \frac{\frac{3}{2} x - \frac{-1}{2}}{x^2 - 2x +3} dx</mrow>
            <mrow>\amp  = \frac{3}{4} \int \frac{2x - \frac{2}{3}}{x^2-2x+3} dx = \frac{3}{4} \int \frac{2x - 2 + (2 - \frac{2}{3})} {x^2-2x+3} dx</mrow>
            <mrow>\amp  = \frac{3}{4} \left( \int \frac{2x-2}{x^2-2x+3} dx + \frac{4}{3} \int \frac{1}{x^2-2x+3} dx \right)</mrow>
            <mrow>\amp  = \frac{3}{4} \ln |x^2-2x+3| + \int \frac{1}{(x-1)^2 +2} dx = \frac{3}{4} \ln |x^2-2x+3| + \frac{1}{\sqrt{2}} \arctan \left( \frac{x-1}{\sqrt{2}} \right)</mrow>
          </md>
        </p>
        <p>
          The whole integral is now complete.
          <me>
            \int \frac{x^2-x-1}{x^3-3x^2+5x-3} dx = \frac{-1}{2} \ln |x-1| + \frac{3}{4} \ln |x^2-2x+3| + \frac{1}{\sqrt{2}} \arctan \left( \frac{x-1}{\sqrt{2}} \right) + c
          </me>
        </p>
      </statement>
    </example>
    <p>
      It's useful to have a reference for the process for these quadratic integrals.
      The previous example showed us the general approach:
      seperate the integral into two pieces,
      a substitution piece and an arctangent piece.
      Consider the general case.
      <me>
        \int \frac{x + c}{x^2 + ax + b}
      </me>
    </p>
    <p>
      The derivative of the denominator is <m>2x + a</m>,
      so we can to manipulate the numerator to make that expression.
      <md>
        <mrow>\int \frac{x + c}{x^2 + ax + b} \amp  = \frac{1}{2} \int \frac{2x + 2c}{x^2 + ax + b} dx</mrow>
        <mrow>\amp  = \frac{1}{2} \int \frac{(2x + a) + (c-a)}{x^2 + ax + b} dx \amp  = \frac{1}{2} \int \frac{2x+a}{x^2 + ax+ b} dx + \frac{c-a}{2} \int \frac{1}{x^2 + ax + b} dx</mrow>
      </md>
    </p>
    <p>
      Then we can do both integrals.
      The substitition integral uses <m>u = x^2 + ax + b</m>.
      <me>
        \int \frac{2x + a}{x^2 + ax + b} dx = \ln |x^2 + ax + b|
      </me>
    </p>
    <p>
      In the second integral, we need to complete the square.
      Once we do, we can use the following general form for arctangent integrals.
      <me>
        \int \frac{1}{(x-\alpha)^2 + \beta^2} dx = \frac{1}{\beta} \arctan \left( \frac{x-\alpha}{\beta} \right) + C
      </me>
    </p>
  </subsection>
  <subsection xml:id="repeated-linear-factors">
    <title>Repeated Linear Factors</title>
    <p>
      So far, none of our examples have had repeated factors.
      Repeated factors change the process a bit.
      By themselves,
      linear repeated factors are still reasonable to integrate.
      <me>
        \int \frac{3}{(x-2)^2} dx = \int \frac{3}{u^3} dx = \frac{-3}{2u^2} + c = \frac{-3}{2 (x-2)^2} + c
      </me>
    </p>
    <p>
      (For repeated quadratic factors the situation is trickier.
      We need reduction formulas or clever manipulations and substitutions.
      For this course, we will ignore repeated quadratic factors.)
    </p>
    <p>
      For a repeated linear factor <m>(x-\alpha)^n</m>,
      we will look for partial fractions with the following denominators.
      <me>
        \frac{a_1}{(x-\alpha)} + \frac{a_2}{(x-\alpha)^2} + \frac{a_3}{(x-\alpha)^3} + \ldots + \frac{a_n}{(x-\alpha)^n} +
      </me>
    </p>
    <example>
      <statement>
        <me>
          \int \frac{2x-3}{(x-1)(x+2)^2}dx
        </me>
        <p>
          To account for the repeated root,
          we look for a partial fraction decomposition of the following form.
          <md>
            <mrow>\frac{2x-3}{(x-1)(x+2)^2} \amp  = \frac{a}{x-1} + \frac{b}{x+2} + \frac{c}{(x+2)^2}</mrow>
            <mrow>\amp  = \frac{a(x+2)^2 + b(x+2)(x-1) + c(x-1)} {(x-1)(x-2)^2}</mrow>
            <mrow>\amp  = \frac{ax^2 + 4ax + 4a + bx^2 + bx - 2b + cx -x } {(x-1)(x-2)^2}</mrow>
            <mrow>\amp  = \frac{(a+b)x^2 + (4a+b+c)x + (4a-2b-c)} {(x-1)(x-2)^2}</mrow>
          </md>
        </p>
        <p>
          We get a system of equations.
          <md>
            <mrow>a+b \amp  = 0</mrow>
            <mrow>4a + b + c \amp  = 2</mrow>
            <mrow>4a-2b-c \amp  = -3</mrow>
          </md>
        </p>
        <p>
          We solve the system.
          <md>
            <mrow>a \amp  = -b</mrow>
            <mrow>\amp  \text{ Substitute this into the second equation }</mrow>
            <mrow>4a + (-a) + c \amp  = 2</mrow>
            <mrow>3a + c \amp  = 2</mrow>
            <mrow>a \amp  = \frac{2-c}{3}</mrow>
            <mrow>\amp  \text{ Substitute this into the third equation }</mrow>
            <mrow>4a - 2b - c \amp  = -3</mrow>
            <mrow>4 \frac{2-c}{3} - 2 \frac{c-2}{3} - c \amp  = -3</mrow>
            <mrow>8 - 4x - 2c + 4 - 3c \amp  = -9</mrow>
            <mrow>-9c \amp  = -21</mrow>
            <mrow>c \amp  = \frac{7}{3}</mrow>
            <mrow>a \amp  = \frac{2 - \frac{7}{3}}{3} = \frac{-1}{9}</mrow>
            <mrow>b \amp  = -a = \frac{1}{9}</mrow>
          </md>
        </p>
        <p>
          Then we can complete the integral.
          <md>
            <mrow>\int \frac{2x-3}{(x-1)(x+2)^2}dx \amp  = \frac{-1}{9} \int \frac{1}{x-1} dx + \frac{1}{9} \int \frac{1}{x+2} dx + \frac{7}{3} \int \frac{1}{(x+2)^2}dx</mrow>
            <mrow>\amp  = \frac{-1}{9} \ln |x-1| + \frac{1}{9} \ln |x+2| + \frac{7}{3} \frac{-1}{x+2} + c</mrow>
          </md>
        </p>
      </statement>
    </example>
    <example>
      <statement>
        <p>
          If we have higher powers of repeated roots,
          we have additional terms in the decomposition.
          We would start a difficult degree seven example with the following decomposition.
          <me>
            \frac{1}{(x+1)(x^2+4)^3} = \frac{a}{x+1} + \frac{bx+c}{x^2+4} + \frac{dc + e}{(x^2+4)^2} + \frac{fx+g}{(x^2+4)^3}
          </me>
        </p>
        <p>
          The resulting system would a a system of seven equations and seven variables,
          which would be laborious to solve.
          (Computers, thankfully,
          are very good at solving system of linear equations.)
        </p>
      </statement>
    </example>
  </subsection>
</section>
