<section xml:id="section-trig-substitutions">
  <title>Trigonometric Substitutions</title>
  <p>
    The last major technique for integration is the technique of
    trigonometric substitutions. While these are technically just a
    new type of substitution, and we already know how to do
    substitution, they are a very counter-intuitive class of
    substitutions which deserve their own section.
  </p>
  <p>
    If <m>x</m> is the indepedant variable and <m>a</m> is a constant,
    trigonometric substitutions are used for integrals that involve
    terms like <m>\sqrt{a^2 - x^2}</m>, <m>\sqrt{x^2 - a^2}</m> and
    <m>\sqrt{x^2 + a^2}</m>. This might seem like very specific set
    of integrands to worry about. However, the ubiquitous presence of
    the pythagorean theorem in geometric arguments leads to many
    integrands of this form.
  </p>
  <p>
    So why trigonometry? The idea is to use the square identities
    <m>\cos^2 x + \sin^2 x = 1</m>, <m>1 + \tan^2 x = \sec^2 x</m> and
    <m>\cot^2 x + 1 = \csc^2 x</m> to simplify the <m>\sqrt{a^2 \pm
    x^2}</m> terms.
  </p>
  <p>
    The following chart outlines the three cases and the appropriate
    trig substitution. In each case, the chart give the term involved
    in the integrand, the appropriate substitution, the trig identity
    that the substitution relies on, the calculation that removes the
    square root term and the domain of application of the
    substitution.
    <md>
      <mrow>
        \text{ Integrand }  \hspace{1cm} \amp \sqrt{a^2 - x^2}
      </mrow>
      <mrow>
        \text{ Substitution }  \hspace{1cm} \amp x = a \sin \theta
      </mrow>
      <mrow>
        \text{ Identity }  \hspace{1cm} \amp \sin^2 \theta + \cos^2
        \theta = 1
      </mrow>
      <mrow>
        \text{ Calculation }  \hspace{1cm} \amp \sqrt{a^2 - x^2} =
        \sqrt{a^2(1-\sin^2 \theta)} = a \cos \theta
      </mrow>
      <mrow>
        \text{ Domain }  \hspace{1cm} \amp \frac{-\pi}{2} \leq \theta
        \leq \frac{\pi}{2}
      </mrow>
      <mrow>
        \text{ Integrand }  \hspace{1cm} \amp \sqrt{a^2 + x^2}
      </mrow>
      <mrow>
        \text{ Substitution }  \hspace{1cm} \amp x = a \tan \theta
      </mrow>
      <mrow>
        \text{ Identity }  \hspace{1cm} \amp \tan^2 \theta + 1 =
        \sec^2 \theta
      </mrow>
      <mrow>
        \text{ Calculation }  \hspace{1cm} \amp \sqrt{a^2 + x^2} =
        \sqrt{a^2(1+\tan^2 \theta)} = a \sec \theta
      </mrow>
      <mrow>
        \text{ Domain }  \hspace{1cm} \amp \frac{-\pi}{2} \leq \theta
        \leq \frac{\pi}{2}
      </mrow>
      <mrow>
        \text{ Integrand }  \hspace{1cm} \amp \sqrt{x^2 - a^2}
      </mrow>
      <mrow>
        \text{ Substitution }  \hspace{1cm} \amp x = a \sec \theta
      </mrow>
      <mrow>
        \text{ Identity }  \hspace{1cm} \amp \tan^2 \theta + 1 =
        \sec^2 \theta
      </mrow>
      <mrow>
        \text{ Calculation }  \hspace{1cm} \amp \sqrt{x^2 - a^2} =
        \sqrt{a^2(\sec^2 \theta - 1)} = a \tan \theta
      </mrow>
      <mrow>
        \text{ Domain }  \hspace{1cm} \amp 0 \leq \theta \leq
        \frac{\pi}{2}
      </mrow>
    </md>
  </p>
  <example>
    <statement>
      <p>
        In the first example, we have to remove a constant from the
        square root to recognize the <m>\sqrt{a^2 - x^2}</m> form.
        <md>
          <mrow>
            \int \sqrt{1-4x^2} dx \amp = 2 \int \sqrt{\frac{1}{4} -
            x^2} dx
          </mrow>
          <mrow>
            \text{ Substitution: }  \amp
          </mrow>
          <mrow>
            \amp x = \frac{1}{2} \sin \theta
          </mrow>
          <mrow>
            \amp dx = \frac{1}{2} \cos \theta d \theta
          </mrow>
          <mrow>
            \text{ Calculation: }  \amp
          </mrow>
          <mrow>
            \amp \sqrt{\frac{1}{4} - x^2} = \sqrt{\frac{1}{4} -
            \frac{\sin^2 \theta}{4}} = \frac{1}{2} \sqrt{1 - \sin^2
            \theta} = \frac{1}{2} \cos \theta
          </mrow>
          <mrow>
            \text{ New Integral: }  \amp
          </mrow>
          <mrow>
            \int \sqrt{1-4x^2} dx \amp = 2 \int \frac{1}{2} \cos
            \theta \frac{1}{2} \cos \theta d \theta
          </mrow>
          <mrow>
            \amp = \frac{1}{2} \int \cos^2 \theta d\theta
          </mrow>
          <mrow>
            \amp = \frac{1}{2} \int \frac{1 + \cos 2 \theta}{2}
            d\theta
          </mrow>
          <mrow>
            \amp = \frac{1}{4} \int d \theta + \int \frac{1}{4} \cos
            2 \theta d\theta
          </mrow>
          <mrow>
            \amp = \frac{\theta}{4} + \frac{\sin 2\theta}{8} + c
          </mrow>
          <mrow>
            \text{ Reverse Substitution: }  \amp
          </mrow>
          <mrow>
            \amp = \frac{\theta}{4} + \frac{2 \sin \theta \cos
            \theta}{8} + c
          </mrow>
          <mrow>
            \amp = \frac{\arcsin 2x}{4} + \frac{2\cdot 2x
            \sqrt{1-4x^2}}{8} + c
          </mrow>
          <mrow>
            \amp = \frac{\arcsin 2x}{4} + \frac{x\sqrt{1-4x^2}}{2} +
            c
          </mrow>
        </md>
      </p>
    </statement>
  </example>
  <example>
    <statement>
      <md>
        <mrow>
          \int \frac{\sqrt{x^2-9}}{x^3} dx \amp
        </mrow>
        <mrow>
          \text{ Substitution: }  \amp
        </mrow>
        <mrow>
          x \amp = 3 \sec \theta
        </mrow>
        <mrow>
          dx \amp = 3 \sec \theta \tan \theta d \theta
        </mrow>
        <mrow>
          \text{ Calculation: }  \amp
        </mrow>
        <mrow>
          \sqrt{x^2-9} \amp = 3 \sqrt{\sec^2 \theta - 1} = 3 \tan
          \theta
        </mrow>
        <mrow>
          \cos \theta \amp = \frac{3}{x}
        </mrow>
        <mrow>
          \sin \theta \amp = \sqrt{1 - \frac{9}{x^2}}
        </mrow>
        <mrow>
          \text{ New Integral: }  \amp
        </mrow>
        <mrow>
          \int \frac{\sqrt{x^2-9}}{x^3} dx \amp = \int \frac{\sqrt{9
          \sec^2 \theta - 9}}{27 \sec^3 \theta} 3 \sec \theta \tan
          \theta d \theta.
        </mrow>
        <mrow>
          \amp = \frac{1}{3} \int \frac{\tan^2
        \theta}{\sec^2 \theta} d \theta
        </mrow>
        <mrow>
          \amp = \frac{1}{3} \int \sin^2 \theta d\theta
        </mrow>
        <mrow>
          \amp = \frac{1}{3} \int
        \frac{1-\cos 2\theta}{2} d \theta
        </mrow>
        <mrow>
          \amp = \frac{1}{3} \int \frac{1}{2} d \theta - \frac{1}{3}
          \int \frac{\cos 2\theta}{2} d\theta
        </mrow>
        <mrow>
          \amp = \frac{\theta}{6} - \frac{\sin 2\theta}{12} + c
        </mrow>
        <mrow>
          \amp = \frac{\theta}{6} - \frac{2 \sin \theta \cos
          \theta}{12} + c
        </mrow>
        <mrow>
          \text{ Reverse Substitution: }  \amp
        </mrow>
        <mrow>
          \amp = \frac{\arcsec\left(\frac{x}{3} \right)}{6} -
          \frac{1}{6} \sqrt{1 - \frac{9}{x^2}} \frac{3}{x} + c
        </mrow>
        <mrow>
          \amp = \frac{\arcsec\left(\frac{x}{3} \right)}{6} -
          \frac{\sqrt{x^2-9}}{2x^2} + c
        </mrow>
      </md>
    </statement>
  </example>
  <example>
    <statement>
      <p>
        Here is an example with bounds. This particular example is
        quite useful: it calculates the area of the ellipse
        <m>\frac{x^2}{a^2} + \frac{y^2}{b^2} = 1</m>. It restricts to
        the quarter of the ellipse in the first quadrant, where the
        area is the area under the curve <m>y = \frac{b}{a}
        \sqrt{a^2-x^2}</m> for <m>x \in [0,a]</m>. Working with the
        bounds is difficult: to get the new bounds in <m>\theta</m>,
        we have to invert the trig functions. Remember the standard
        choices for inverting trig functions, or simply work by
        intuition. Using special triangles is often convenient.
        <md>
          <mrow>
            A \amp = 4 \int_0^a \frac{b}{a} \sqrt{a^2-x^2} dx
          </mrow>
          <mrow>
            \text{ Substitution: }  \amp
          </mrow>
          <mrow>
            \amp x = a \sin \theta
          </mrow>
          <mrow>
            \amp dx = a \cos \theta d \theta
          </mrow>
          <mrow>
            \text{ Bounds: }  \amp
          </mrow>
          <mrow>
            \amp x = 0 \implies \theta = 0
          </mrow>
          <mrow>
            \amp x = a \implies \theta = \frac{\pi}{2}
          </mrow>
          <mrow>
            \text{ New Integral: }  \amp
          </mrow>
          <mrow>
            A \amp = 4 \int_0^{\frac{\pi}{2}} \frac{b}{a} \sqrt{a^2 -
            a^2 \sin^2 \theta} a \cos \theta d \theta
          </mrow>
          <mrow>
            \amp = \frac{4ba^2}{a} \int_0^{\frac{\pi}{2}} \cos^2
            \theta d\theta
          </mrow>
          <mrow>
            \amp = 4ab \int_0^{\frac{\pi}{2}} \frac{1 + \cos
            2\theta}{2} d\theta
          </mrow>
          <mrow>
            \amp = \frac{4ab}{2} \left( \int_0^{\frac{\pi}{2}} 1
            d\theta + \int_0^{\frac{\pi}{2}} \cos 2\theta d\theta
            \right)
          </mrow>
          <mrow>
            \amp = \frac{2ab\pi}{2} + \left. 2ab\frac{\sin
            2\theta}{2} \right|_0^{\frac{\pi}{2}} = \pi ab + 0 - 0 =
            \pi ab
          </mrow>
        </md>
      </p>
      <p>
        Therefore, the area of an ellipse with major axis <m>a</m> and
        minor axis <m>b</m> is <m>\pi ab</m>. This notion of area
        reduces to the area of a circle, where <m>a=b</m> and we get
        <m>\pi a^2</m> for <m>a</m> the radius.
      </p>
    </statement>
  </example>
  <example>
    <statement>
      <p>
        Here is another long example with bounds.
        <md>
          <mrow>
            \int_{\frac{\sqrt{2}}{3}}^{\frac{2}{3}}
            \frac{dx}{x^5\sqrt{9x^2-1}} \amp =
            \int_{\frac{\sqrt{2}}{3}}^{\frac{2}{3}}
            \frac{dx}{3x^5\sqrt{x^2 - \frac{1}{9}}}
          </mrow>
          <mrow>
            \amp u = \frac{1}{3} \sec \theta
          </mrow>
          <mrow>
            \amp du = \frac{1}{3} \sec \theta \tan \theta d \theta
          </mrow>
          <mrow>
            \amp u = \frac{\sqrt{2}}{3} \implies \sec \theta =
            \sqrt{2} \implies \cos \theta = \frac{1}{\sqrt{2}}
            \implies \theta = \frac{\pi}{4}
          </mrow>
          <mrow>
            \amp u = \frac{2}{3} \implies \sec \theta = 2 \implies
            \cos \theta = \frac{1}{2} \implies \theta = \frac{\pi}{3}
          </mrow>
          <mrow>
            \int_{\frac{\sqrt{2}}{3}}^{\frac{2}{3}} \frac{dx}{3x^5
            \sqrt{x^2 - \frac{1}{9}}} \amp =
            \int_{\frac{\pi}{4}}^{\frac{\pi}{3}} \frac{\frac{1}{3}
            \sec \theta \tan \theta d\theta}{3 \frac{\sec^5
            \theta}{3^5} \sqrt{\frac{\sec^2 \theta}{9} -
            \frac{1}{9}}}
          </mrow>
          <mrow>
            \amp = \int_{\frac{\pi}{4}}^{\frac{\pi}{3}}
            \frac{3^6}{3^2} \frac{\tan \theta}{\sec^4 \theta \tan
            \theta} d \theta
          </mrow>
          <mrow>
            \amp = 81 \int_{\frac{\pi}{4}}^{\frac{\pi}{3}} \cos 4
            \theta d \theta
          </mrow>
          <mrow>
            \amp = 81 \int_{\frac{\pi}{4}}^{\frac{\pi}{3}} \left(
            \frac{1 + \cos 2\theta}{2} \right)^2 d \theta
          </mrow>
          <mrow>
            \amp = 81 \left( \int_{\frac{\pi}{4}}^{\frac{\pi}{3}}
            \frac{1}{4} d\theta + \int_{\frac{\pi}{4}}^{\frac{\pi}{3}}
            \frac{\cos 2\theta}{2} d \theta +
            \int_{\frac{\pi}{4}}^{\frac{\pi}{3}} \frac{\cos^2 2
            \theta}{4} d\theta \right)
          </mrow>
          <mrow>
            \amp = 81 \left( \frac{\frac{\pi}{3} - \frac{\pi}{4}}{4}
            + \left. \frac{\sin 2\theta}{4}
            \right|_{\frac{\pi}{4}}^{\frac{\pi}{3}} +
            \int_{\frac{\pi}{4}}^{\frac{\pi}{3}} \frac{\cos^2
            2\theta}{4} d \theta \right)
          </mrow>
          <mrow>
            \amp = 81 \left(\frac{\pi}{48} + \frac{\sqrt{3}}{8} -
            \frac{1}{4} + \int_{\frac{\pi}{4}}^{\frac{\pi}{3}}
            \frac{1}{8} d\theta + \int_{\frac{\pi}{4}}^{\frac{\pi}{3}}
            \frac{1 + \cos 4\theta}{8} d\theta \right)
          </mrow>
          <mrow>
            \amp = 81 \left(\frac{\pi}{48} + \frac{\sqrt{3}}{8} -
            \frac{1}{4} + \frac{\pi}{96} + \left. \frac{\sin
            4\theta}{32} \right|_{\frac{\pi}{4}}^{\frac{\pi}{3}}
            \right)
          </mrow>
          <mrow>
            \amp = 81 \left(\frac{\pi}{48} + \frac{\pi}{96}
            \frac{\sqrt{3}}{8} - \frac{1}{4} - \frac{\sqrt{3}}{64} + 0
            \right)
          </mrow>
          <mrow>
            \amp = 81 \left( \frac{2\pi + \pi}{96} + \frac{8\sqrt{3}
            - \sqrt{3}}{64} - \frac{1}{4} \right) = 81 \left(
            \frac{3\pi}{96} + \frac{7\sqrt{3}}{64} - \frac{16}{64}
            \right)
          </mrow>
          <mrow>
            \amp = 81 \left( \frac{\pi}{32} + \frac{7\sqrt{3} -
            16}{64} \right) = \frac{81}{64} ( 2\pi + 7\sqrt{3} - 16)
          </mrow>
        </md>
      </p>
    </statement>
  </example>
</section>
