<section xml:id="section-week6-activity">
  <title>Week 6 Activity</title>
  <subsection xml:id="subsection-activity-">
    <title>Title</title>
    <activity>
      <statement>
        <p>
          Question
        </p>
      </statement>
      <solution>
        <p>
          Solution
        </p>
      </solution>
    </activity>
  </subsection>
  <subsection xml:id="subsection-week6-concepts">
    <title>Conceptual Review Questions</title>
    <p>
      <ul>
        <li>
          Question
        </li>
      </ul>
    </p>
  </subsection>
  <subsection xml:id="subsection-week6-extra-practice">
    <title>Extra Practice Activities</title>
    <activity>
      <statement>
        <p>
          Question
        </p>
      </statement>
      <solution>
        <p>
          Solution
        </p>
      </solution>
    </activity>
  </subsection>
</section>


  \item Calculate this integral. Show and annotate the various steps
  in the process. (This is a very long question, so here is some
  guidance. After a trig substitution, you will get a
  trig function cubed. Write this $f^3$ as $f^2 \cdot f$ and use 
  integration by parts. After the integration by parts, change
  everything into sine and cosine and see if a substitution will work.) (8) 
  \begin{equation*}
    \int \frac{x^2}{\sqrt{x^2-9}} dx \\
  \end{equation*}
  The precense of the square root indicates that a trig substitution
  will be the best approach. Consulgin the table, I need a secant
  substitution. I proceed to setup the pieces of the substitution.  
  \begin{align*}
    x & = 3 \sec \theta \\
    dx & = 3 \sec \theta \tan \theta d \theta \\
    \sqrt{x^2 - 9} & = \sqrt{9\sec^2 \theta - 9} = 3\sqrt{\sec^2
    \theta - 1} = 3 \tan \theta 
  \end{align*}
  Then I do the substition. Afer doing the substitution, I simplify
  but leave everything in terms of secant and tangent. 
  \begin{align*}
    \int \frac{x^2}{\sqrt{x^2-9}} dx \\
    & = \int \frac{9 \sec^2 \theta}{3 \tan \theta} 3 \sec \theta
    \tan \theta d \theta \\
    & = 9 \int \sec^3 \theta d \theta 
    & = 9 \int \sec^2 \theta \sec \theta d \theta 
  \end{align*}
  I'm going to try integration by parts with these choices for the two
  pieces of the product.
  \begin{align*}
    g(x)  & = \sec \theta \\
    \frac{df}{dx}  & = \sec^2 \theta \\
    \frac{dg}{dx}  & = \sec \theta \tan \theta \\
    f(x) = \tan \theta 
  \end{align*}
  I made those choices for integration by parts specifically because
  $\sec^2 \theta$ has an easy antiderivative. Now I proceed with
  integration by parts. In the remaining integral, I'll change
  everything into sine and cosine, and then even further, changing
  most of the cosines to sines using $\sin^2 \theta + \cos^2 \theta =
  1$. (The term without an integral is finished, so I won't adjust it
  while I adjust the remaining integral.)
  \begin{align*}
    9 \int \sec^2 \theta \sec \theta d \theta 
    & = 9 \sec \theta \tan \theta - 9 \int \sec \theta \tan^2
    \theta d \theta = 9 \sec \theta \tan \theta - 9 \int
    \frac{\sin^2 \theta}{\cos^3 \theta} d \theta \\
    & = 9 \sec \theta \tan \theta - 9 \int \frac{\sin^2
    \theta}{\cos^4 \theta} \cos \theta d \theta = 9 \sec \theta
    \tan \theta - - 9 \int \frac{\sin^2 \theta}{(1-\sin^2
    \theta)^2} \cos \theta d \theta 
  \end{align*}
  Then everything is an expression in sine except for one cosine. A
  substitution using sine here should work. I'll setup the
  substitution. 
  \begin{align*}
    w & = \sin \theta \\
    dw & = \cos \theta d \theta \\
    & = 9 \sec \theta \tan \theta - 9 \int \frac{w}{(1-w^2)^2} dw \\
    y & = 1-w^2 \\
    dy & = -2w dw \implies \frac{-1}{2} dy = w dw \\
    & = 9 \sec \theta \tan \theta - 9 \frac{-1}{2} \int
\frac{1}{y} dy \\
& = 9 \sec \theta \tan \theta + \frac{9}{2} \ln |y| + C \\
& = 9 \sec \theta \tan \theta + \frac{9}{2} \ln |1-w^2| + C \\
& = 9 \sec \theta \tan \theta + \frac{9}{2} \ln |1-\sin^2
\theta| + C \\
& = 9 \sec \theta \tan \theta + \frac{9}{2} \ln |1-\sin^2
\theta| + C \\
& = 9 \sec \theta \tan \theta + \frac{9}{2} \ln |\cos^2 \theta| + C \\
& = 3 \sec \theta 3 \tan \theta + \frac{9}{2} \ln \left|
\frac{1}{\sec^2 \theta} \right| + C \\
& = x \sqrt{x^2-9} + \frac{9}{2} \ln \left|
\frac{9}{x^2} \right| + C \\
\end{align*}
