<section xml:id="section-week12-activity">
  <title>Week 12 Activity</title>
  <subsection xml:id="subsection-activity-radius-convergence">
    <title>Power Series</title>
    <activity>
      <statement>
        <p>
          Determine the radius of convergence and domain of definition
          for this power series.
        </p>
        <me>
          \sum_{n=0}^\infty \frac{n}{n^3 + 1} x^n 
        </me>
      </statement>
      <solution>
        <p>
          I'll use the limit test for this radius of convergence,
          since none of the coefficients are zero. I need to simplify
          the nested fraction, expand the cubed binomial, and evaluate
          the limit asymptotically.
        </p>
        <md>
          <mrow>
            R \amp = \lim_{n \rightarrow \infty} \left|
            \frac{c_n}{c_{n+1}} \right| 
          </mrow>
          <mrow>
            \amp = \lim_{n \rightarrow \infty} \left|
            \frac{\frac{n}{n^3+1}}{\frac{(n+1)}{(n+1)^3+1}} \right| 
          </mrow>
          <mrow>
            \amp = \lim_{n \rightarrow \infty} 
            \frac{n((n+1)^3+1}{(n+1)(n^3+1)} = \lim_{n \rightarrow
            \infty} \frac{n^4 + 3n^3 + 2n + 2}{n^4 + n^3 + n + 1} = 1 
          </mrow>
        </md>
        <p>
          The radius of convergence is <m>R = 1</m>. Since the centre
          point is <m>\alpha = -</m>, the domain of definition is
          <m>(-1,0)</m>.     
        </p>
      </solution>
    </activity>
    <activity>
      <statement>
        <p>
          Determine the radius of convergence and domain of definition
          for this power series.
        </p>
        <me>
          \sum_{n=0}^\infty \frac{1}{n!} (x-4)^n 
        </me>
      </statement>
      <solution>
        <p>
          I'll use the limit test for this radius of convergence,
          since none of the coefficients are zero.
        </p>
        <me>
          R = \lim_{n \rightarrow \infty} \left| \frac{c_n}{c_{n+1}}
          \right| = \lim_{n \rightarrow \infty} \left|
          \frac{\frac{1}{n!}}{\frac{1}{(n+1)!}} \right| = \lim_{n
          \rightarrow \infty} \frac{(n+1)!}{n!} = \lim_{n \rightarrow
          \infty} n = \infty
        </me>
        <p>
          The radius of convergence is <m>R = \infty</m>. The domain
          of definition is all real numbers. 
        </p>
      </solution>
    </activity>
    <activity>
      <statement>
        <p>
          Determine the radius of convergence and domain of definition
          for this power series.
        </p>
        <me>
          \sum_{n=0}^\infty \frac{(-1)^n}{n} (x-3)^n 
        </me>
      </statement>
      <solution>
        <p>
          I'll use the limit test for this radius of convergence,
          since none of the coefficients are zero.
        </p>
        <me>
          R = \lim_{n \rightarrow \infty} \left| \frac{c_n}{c_{n+1}}
          \right| = \lim_{n \rightarrow \infty} \left|
          \frac{\frac{(-1)^n}{n}}{\frac{(-1)^{n+1}}{n+1}} \right| =
          \lim_{n \rightarrow \infty} \frac{n+1}{n} = 1
        </me>
        <p>
          The radius of convergence is <m>R = 1</m>. Since the centre
          point is <m>\alpha = 3</m>, the domain of definition is
          <m>(2,4)</m>.     
        </p>
      </solution>
    </activity>
    <activity>
      <statement>
        <p>
          Determine the radius of convergence and domain of definition
          for this power series.
        </p>
        <me>
          \sum_{n=0}^\infty (\ln n) x^n 
        </me>
      </statement>
      <solution>
        <p>
          I'll use the limit test for this radius of convergence,
          since none of the coefficients are zero. I'll use
          L'Hôpital's rule for this limit, which conveniently gets
          rid of the logarithms. (The limit has type
          <m>\frac{\infty}{\infty}</m>, so L'Hôpital's rule is
          justified.
        </p>
        <me>
          R = \lim_{n \rightarrow \infty} \left| \frac{c_n}{c_{n+1}}
          \right| = \lim_{n \rightarrow \infty} \left| \frac{\ln
          n}{\ln (n+1)} \right| = \lim_{n \rightarrow \infty}
          \frac{\frac{1}{n}}{\frac{1}{n+1}} = \lim_{n \rightarrow
          \infty} \frac{n+1}{n} = 1
        </me>
        <p>
          The radius of convergence is <m>R = 1</m>. Since the centre
          point is <m>\alpha = 0</m>, the domain of definition is
          <m>(-1,1)</m>.     
        </p>
      </solution>
    </activity>
    <activity>
      <statement>
        <p>
          Determine the radius of convergence and domain of definition
          for this power series.
        </p>
        <me>
          \sum_{n=0}^\infty \frac{1}{n!} x^{2n} 
        </me>
      </statement>
      <solution>
        <p>
          This series has only even terms; all the odd terms are zero.
          Since there are even terms, a direct use of either the limit
          calculation for the radius of convergence or the ratio test
          leads to division by zero problems. However, I can adjust a
          bit. I can think of this as a power series in <m>x^2</m>. If
          I do that, then all the terms are non-zero and I can use the
          limit. The result will give a radius that applies to
          <m>x^2</m>. Here is the limit.
        </p>
        <me>
          R = \lim_{n \rightarrow \infty} \left| \frac{c_n}{c_{n+1}}
          \right| = \lim_{n \rightarrow \infty} \left|
          \frac{\frac{1}{n!}}{\frac{1}{(n_1)!}} \right| = \lim_{n
          \rightarrow \infty} \frac{(n+1)!}{n!} = \lim_{n \rightarrow
          \infty} n+1 = \infty
        </me>
        <p>
          The radius of convergence is <m>R = \infty</m>. Therefore,
          the series is defined everywhere. Technically, since I made
          this a series in <m>x^2</m>, the limit shows that <m>x^2</m>
          can be any real number. That immediatly implies that the
          original input <m>x</m> can be any real number as well. 
        </p>
      </solution>
    </activity>
    <activity>
      <statement>
        <p>
          Determine the radius of convergence and domain of definition
          for this power series.
        </p>
        <me>
          \sum_{n=0}^\infty \frac{n!(n+2)!}{(2n+3)!} (x+2)^n 
        </me>
      </statement>
      <solution>
        <p>
          I'll use the limit test for this radius of convergence,
          since none of the coefficients are zero. This limit is all
          about factorial algebra. I'll simplify the nested fraction
          and then group similar factorial terms together. Then I'll
          cancel the factorials and look at the remaining polynomial
          terms. 
        </p>
        <md>
          <mrow>
            R \amp = \lim_{n \rightarrow \infty} \left|
            \frac{c_n}{c_{n+1}} \right| = \lim_{n \rightarrow \infty}
            \frac{\frac{n!(n+2)!}{(2n+3)!}}{\frac{(n+1)!(n+3)!}{(2n+5)!}}
          </mrow>
          <mrow>
            \amp = \lim_{n \rightarrow \infty} \frac{n!}{(n+1)!}
            \frac{(n+2)!}{(n+3)!} \frac{(2n+5)!}{(2n+3)!} 
          </mrow>
          <mrow>
            \amp = \lim_{n \rightarrow \infty}
            \frac{(2n+4)(2n+5)}{(n+1)(n+3)} 
            = \lim{n \rightarrow \infty}
            \frac{4n^2 + 18n + 20}{n^2 + 4n + 3} = 4 
          </mrow>
        </md>
        <p>
          After simplifying the factorial, the limit is a quadratic in
          both the denominator and numerator. Since these have the
          same asymptotic order, the limit is the ratio of the leading
          coefficients.  The radius of convergence is <m>R = 4</m>.
          Since the centre point is <m>\alpha = 0</m>, the domain of
          definition is <m>(-4,4)</m>.     
        </p>
      </solution>
    </activity>
  </subsection>
  <subsection xml:id="subsection-activity-taylor-series">
    <activity>
      <statement>
        <p>
          Calculate the Taylor series for <m>f(x) = \cosh x</m> with
          centre point <m>x = 0</m>. Determine its radius of
          convergence. 
        </p>
      </statement>
      <solution>
        <p>
          First I need the derivatives of the function. I'll take the
          first few derivatives.
        </p>
        <md>
          <mrow>
            f(x) \amp = \cosh x 
          </mrow>
          <mrow>
            \frac{d}{dx} f(x) \amp = \sinh x 
          </mrow>
          <mrow>
            \frac{d^2}{dx^2} f(x) \amp = \cosh x
          </mrow>
          <mrow>
            \frac{d^3}{dx^3} f(x) \amp = \sinh x 
          </mrow>
          <mrow>
            \frac{d^4}{dx^4} f(x) \amp = \cosh x
          </mrow>
          <mrow>
            \frac{d^5}{dx^5} f(x) \amp = \sinh x 
          </mrow>
          <mrow>
            \frac{d^6}{dx^6} f(x) \amp = \cosh x
          </mrow>
        </md>
        <p>
          Then I'll evaluate at the centre point. 
        </p>
        <md>
          <mrow>
            f(0) \amp = 1
          </mrow>
          <mrow>
            \frac{d}{dx} f(x) \Bigg|_{x=0} \amp = 0
          </mrow>
          <mrow>
            \frac{d^2}{dx^2} f(x) \Bigg|_{x=0} \amp = 1
          </mrow>
          <mrow>
            \frac{d^3}{dx^3} f(x) \Bigg|_{x=0} \amp = 0
          </mrow>
          <mrow>
            \frac{d^4}{dx^4} f(x) \Bigg|_{x=0} \amp = 1
          </mrow>
          <mrow>
            \frac{d^5}{dx^5} f(x) \Bigg|_{x=0} \amp = 0
          </mrow>
          <mrow>
            \frac{d^6}{dx^6} f(x) \Bigg|_{x=0} \amp = 1
          </mrow>
        </md>
        <p>
          Then I need to find a pattern. Here, the pattern is
          relatively obvious: a sequences of alternating zeros and
          ones. Only the even terms are non-zero, so I'll only write
          the even terms in the final Taylor series. To write the even
          terms, I use <m>(2n)</m> as <m>n \in \NN</m>.
        </p>
        <me>
          \frac{d^{2n}}{dx^{2n}} f(x) \Bigg|_{x=0} = 1 
        </me>
        <p>
          After describing a pattern for the derivatives at the centre
          point, I put that pattern into the standard form of the
          Taylor series. 
        </p>
        <me>
          f(x) = \sum_{n=0}^\infty \frac{1}{(2n)!} x^{2n} 
        </me>
        <p>
          I take the limit of the ration of the coefficients to
          determine the radius of convergence. (In this case, since
          there are only even terms, the resulting radius will be a
          bound on <m>x^2</m> instead of <m>x</m>.)
        </p>
        <me>
          R = \lim_{n \rightarrow \infty} \left| \frac{c_n}{c_{n+1}}
          \right| = \lim_{n \rightarrow \infty} \left|
          \frac{\frac{1}{n!}}{\frac{1}{(n+1)!}} \right| = \lim_{n
          \rightarrow \infty} \frac{(n+1)!}{n!} = \lim_{n \rightarrow
          \infty} n+1 = \infty
        </me>
        <p>
          The radius of convergence for <m>x^2</m> is <m>R =
          \infty</m>. Since <m>x^2</m> can be any real number,
          <m>x</m> can also be any real number, to the radius of
          convergence for the series is, indeed, infinity. 
        </p>
      </solution>
    </activity>
    <activity>
      <statement>
        <p>
          Calculate the Taylor series for <m>f(x) = \frac{1}{x}</m>
          with centre point <m>x = 1</m>. Determine its radius of
          convergence. 
        </p>
      </statement>
      <solution>
        <p>
          First I need the derivatives of the function. I'll take the
          first few derivatives.
        </p>
        <md>
          <mrow>
            f(x) \amp = \frac{1}{2} 
          </mrow>
          <mrow>
            \frac{d}{dx} f(x) \amp = \frac{-1}{x^2} 
          </mrow>
          <mrow>
            \frac{d^2}{dx^2} f(x) \amp = \frac{2}{x^3} 
          </mrow>
          <mrow>
            \frac{d^3}{dx^3} f(x) \amp = \frac{-(2)(3)}{x^4}
          </mrow>
          <mrow>
            \frac{d^4}{dx^4} f(x) \amp = \frac{(2)(3)(4)}{x^5} 
          </mrow>
          <mrow>
            \frac{d^5}{dx^5} f(x) \amp = \frac{-(2)(3)(4)(5)}{x^6}
          </mrow>
          <mrow>
            \frac{d^6}{dx^6} f(x) \amp = \frac{(2)(3)(4)(5)(6)}{x^7}
          </mrow>
        </md>
        <p>
          Then I'll evaluate at the centre point. 
        </p>
        <md>
          <mrow>
            f(0) \amp = 1
          </mrow>
          <mrow>
            \frac{d}{dx} f(x) \Bigg|_{x=0} \amp = -1
          </mrow>
          <mrow>
            \frac{d^2}{dx^2} f(x) \Bigg|_{x=0} \amp = 2
          </mrow>
          <mrow>
            \frac{d^3}{dx^3} f(x) \Bigg|_{x=0} \amp = -(2)(3)
          </mrow>
          <mrow>
            \frac{d^4}{dx^4} f(x) \Bigg|_{x=0} \amp = (2)(3)(4)
          </mrow>
          <mrow>
            \frac{d^5}{dx^5} f(x) \Bigg|_{x=0} \amp = -(2)(3)(4)(5)
          </mrow>
          <mrow>
            \frac{d^6}{dx^6} f(x) \Bigg|_{x=0} \amp = (2)(3)(4)(5)(6)
          </mrow>
        </md>
        <p>
          Then I need to find a pattern. The sign is alternating, so I
          need a power of <m>(-1)</m>. Since the even terms are
          positive, <m>(-1)^n</m> will work. After the sign, it looks
          like I'm building a factorial. The degree of the derivative
          matches the degree of the factorial. 
        </p>
        <me>
          \frac{d^n}{dx^n} f(x) \Bigg|_{x=0} = (-1)^n n!
        </me>
        <p>
          After describing a pattern for the derivatives at the centre
          point, I put that pattern into the standard form of the
          Taylor series. 
        </p>
        <me>
          f(x) = \sum_{n=0}^\infty \frac{(-1)^n n!}{n!} (x-1)^n =
          \sum_{n=0}^\infty (-1)^n (x-1)^n 
        </me>
        <p>
          I take the limit of the ration of the coefficients to
          determine the radius of convergence.  
        </p>
        <me>
          R = \lim_{n \rightarrow \infty} \left| \frac{c_n}{c_{n+1}}
          \right| = \lim_{n \rightarrow \infty} \left|
          \frac{(-1)^n}{(-1)^{n+1}} \right| = \lim_{n \rightarrow
          \infty} 1 = 1 
        </me>
        <p>
          The radius of convergence is <m>R = 1</m>. 
        </p>
      </solution>
    </activity>
    <activity>
      <statement>
        <p>
          Calculate the Taylor series for <m>f(x) = x^7 + 8x^6 - 19x^5
          + 12x^4 + 3x^3 - 19x^2 + 4x + 41 </m> with
          centre point <m>x = 0</m>. Determine its radius of
          convergence. 
        </p>
      </statement>
      <solution>
        <p>
          This is a bit of a trick question. A polynomial is already
          in the form of a Taylor series centred at <m>\alpha =
          0</m>. Since series representations are unique, there is no
          other way to write this polynomial as a series. There is
          nothing to do here. If you did do the steps, you would
          recover exactly the same expression and you would find that
          all coefficients for <m>x^8</m> and above would be zero. The
          radius of convergence is <m>\infty</m>, since a polynomial
          is defined everywhere. 
        </p>
      </solution>
    </activity>
    <activity>
      <statement>
        <p>
          Calculate the Taylor series for <m>f(x) = \ln (x+3)</m> with
          centre point <m>x = 0</m>. Determine its radius of
          convergence. 
        </p>
      </statement>
      <solution>
        <p>
          First I need the derivatives of the function. I'll take the
          first few derivatives.
        </p>
        <md>
          <mrow>
            f(x) \amp = \ln (x+3)
          </mrow>
          <mrow>
            \frac{d}{dx} f(x) \amp = \frac{1}{x+3}
          </mrow>
          <mrow>
            \frac{d^2}{dx^2} f(x) \amp = \frac{-1}{(x+3)^2}
          </mrow>
          <mrow>
            \frac{d^3}{dx^3} f(x) \amp = \frac{-2}{(x+3)^3} 
          </mrow>
          <mrow>
            \frac{d^4}{dx^4} f(x) \amp = \frac{((2)(3)}{(x+3)^4}
          </mrow>
          <mrow>
            \frac{d^5}{dx^5} f(x) \amp = \frac{-(2)(3)(4)}{(x+3)^5}
          </mrow>
          <mrow>
            \frac{d^6}{dx^6} f(x) \amp = \frac{(2)(3)(4)(5)}{(x+3)^6}
          </mrow>
        </md>
        <p>
          Then I'll evaluate at the centre point. 
        </p>
        <md>
          <mrow>
            f(0) \amp = \ln 3 
          </mrow>
          <mrow>
            \frac{d}{dx} f(x) \Bigg|_{x=0} \amp = \frac{1}{3} 
          </mrow>
          <mrow>
            \frac{d^2}{dx^2} f(x) \Bigg|_{x=0} \amp = \frac{-1}{3^2} 
          </mrow>
          <mrow>
            \frac{d^3}{dx^3} f(x) \Bigg|_{x=0} \amp = \frac{2}{3^3} 
          </mrow>
          <mrow>
            \frac{d^4}{dx^4} f(x) \Bigg|_{x=0} \amp =
            \frac{-(2)(3)}{3^4} 
          </mrow>
          <mrow>
            \frac{d^5}{dx^5} f(x) \Bigg|_{x=0} \amp =
            \frac{(2)(3)(4)}{3^5} 
          </mrow>
          <mrow>
            \frac{d^6}{dx^6} f(x) \Bigg|_{x=0} \amp =
            \frac{-(2)(3)(4)(5)}{3^6} 
          </mrow>
        </md>
        <p>
          Then I need to find a pattern. The signs are alternating and
          the odd terms are positive, so I need <m>(-1)^{n+1}</m>. I
          am buliding a factorial in the numerator, but the degree of
          the factorial is one less than the degree of the
          derivatives, so I'll need <m>(n-1)!</m>. Finally, there is a
          power of <m>3</m> in the numerator and the exponent is the
          same as the degree of the derivative. Also, the first
          term doesn't fit the pattern, so I'll have to remember to
          keep that term seperate. 
        </p>
        <me>
          \frac{d^n}{dx^n} f(x) \Bigg|_{x=0} =
          \frac{(-1)^{n+1}(n-1)!}{3^n} 
        </me>
        <p>
          After describing a pattern for the derivatives at the centre
          point, I put that pattern into the standard form of the
          Taylor series. I need to remember that the first term
          doesn't fit the pattern and must be written apart from the
          sigma notation.
        </p>
        <me>
          f(x) = \ln 3 + \sum_{n=1}^\infty \frac{(-1)^{n+1}(n-1)!}{3^n
          n!} x^n = \ln 3 + \sum_{n=1}^\infty \frac{(-1)^{n+1}}{n3^n} x^n 
        </me>
        <p>
          I take the limit of the ration of the coefficients to
          determine the radius of convergence.  
        </p>
        <me>
          R = \lim_{n \rightarrow \infty} \left| \frac{c_n}{c_{n+1}}
          \right| = \lim_{n \rightarrow \infty} \left|
          \frac{\frac{(-1)^{n+1}}{n3^n}}{\frac{(-1)^{n+2}}{(n+1)3^{n+1}}}
          \right| = \lim_{n \rightarrow \infty}
          \frac{(n+1)3^{n+1}}{n3^n} = \lim_{n \rightarrow \infty}
          3 \frac{n+1}{n} = 3 
        </me>
        <p>
          The radius of convergence is <m>R = 3</m>. 
        </p>
      </solution>
    </activity>
  </subsection>
  <subsection xml:id="subsection-week12-concepts">
    <title>Conceptual Review Questions</title>
    <p>
      <ul>
        <li>
          What is a radius of convergence?
        </li>
      </ul>
      <ul>
        <li>
          How do series represent functions?
        </li>
      </ul>
      <ul>
        <li>
          Why can series define all sorts of new non-elementary
          functions?
        </li>
      </ul>
    </p>
  </subsection>
</section>
